<section xml:id="sec_diff-analytic">
  <title>Differentiable and Analytic Functions</title>
  <p>
    Using our imagination,
    we take our lead from elementary calculus and define the derivative of <m>f</m> at <m>z_0</m>,
    written <m>f\,'(z_0)</m>, by
    <men xml:id="Deriv_Def_1">
      f\,'(z_0) = \lim\limits_{z \to z_0}\frac{f(z) -f(z_0)}{z-z_0}
    </men>,
    provided the limit exists.
    If it does, we say that the function <m>f</m> is
    <term>differentiable at</term><m>z_0</m>.
    If we write <m>\Delta z=z-z_0</m>,
    then we can express Equation <xref ref="Deriv_Def_1"/> in the form
    <men xml:id="Deriv_Def_2">
      f\,'(z_0) = \lim\limits_{\Delta z \to 0}\frac{f(z_0+\Delta z) -f(z_0)}{\Delta z}
    </men>.
  </p>
  <p>
    If we let <m>w=f(z)</m> and <m>\Delta w=f(z)-f(z_0)</m>,
    then we can use the Leibniz notation <m>\frac{dw}{dz}</m> for the derivative:
    <men xml:id="Deriv_Def_3">
      f\,'(z_0) = \frac{dw}{dz}= \lim\limits_{\Delta z \to 0}\frac{\Delta w}{\Delta z}
    </men>.
  </p>
  <example xml:id="DerivEx">
    <statement>
      <p>
        If <m>f(z)=z^3</m>, show that <m>f\,'(z) =3z^2</m>.
      </p>
    </statement>
    <solution>
      <p>
        Using Equation <xref ref="Deriv_Def_1"/>, we have
        <md>
          <mrow>f\,'(z_0) \amp  = \lim_{z \to z_0}\frac{z^3-z_0^3}{z-z_0}</mrow>
          <mrow>\amp = \lim_{z \to z_0}\frac{(z-z_0) (z^2+z_0z+z_0^2)}{z-z_0}</mrow>
          <mrow>\amp = \lim_{z \to z_0}(z^2+z_0z+z_0^2)</mrow>
          <mrow>\amp = 3z_0^2</mrow>
        </md>.
      </p>
      <p>
        We can drop the subscript on <m>z_0</m> to obtain
        <m>f\,'(z) =3z^2</m> as a general formula.
      </p>
    </solution>
  </example>
  <p>
    Pay careful attention to the complex value
    <m>\Delta z</m> in Equation <xref ref="Deriv_Def_3"/>;
    the value of the limit must be independent of the manner in which <m>\Delta z \to 0</m>.
    If we can find two curves that end at <m>z_0</m> along which
    <m>\frac{\Delta w}{\Delta z}</m> approaches distinct values,
    then <m>\frac{ \Delta w}{\Delta z}</m> does <em>not</em>
    have a limit as <m>\Delta z \to 0</m> and <m>f</m> does <em>not</em>
    have a derivative at <m>z_0</m>.
    The same observation applies to the limits in Equations <xref ref="Deriv_Def_2"/> and <xref ref="Deriv_Def_1"/>.
  </p>
  <example>
    <statement>
      <p>
        Show that the function <m>w=f(z) = \overline{z}=x-iy</m> is nowhere differentiable.
      </p>
    </statement>
    <solution>
      <p>
        We choose two approaches to the point
        <m>z_0=x_0+iy_0</m> and compute limits of the difference quotients.
        First, we approach <m>z_0=x_0+iy_0</m> along a line parallel to the <m>x</m>-axis by forcing <m>z</m> to be of the form <m>z=x+iy_0</m>.
        <md>
          <mrow>\lim\limits_{z \to z_0}\frac{f(z) -f(z_0)}{z-z_0} \amp = \lim\limits_{(x+iy_0)  \to (x_0+iy_0)} \frac{f(x+iy_0) - f(x_0+iy_0)}{(x+iy_0)-(x_0+iy_0)}</mrow>
          <mrow>\amp = \lim\limits_{(x+iy_0)  \to (x_0+iy_0)}\frac{(x-iy_0) -(x_0-iy_0)}{(x-x_0) +i(y_0-y_0)}</mrow>
          <mrow>\amp = \lim\limits_{(x+iy_0)  \to (x_0+iy_0)}\frac{x-x_0}{x-x_0}</mrow>
          <mrow>\amp = 1</mrow>
        </md>.
      </p>
      <p>
        Next, we approach <m>z_0</m> along a line parallel to the <m>y</m> axis by forcing <m>z</m> to be of the form <m>z=x_0+iy</m>.
        <md>
          <mrow>\lim_{z \to z_0}\frac{f(z) -f(z_0)}{z-z_0} \amp = \lim\limits_{(x_0+iy)  \to (x_0+iy_0)}\frac{f(x_0+iy) -f(x_0+iy_0)}{(x_0+iy) -(x_0+iy_0)}</mrow>
          <mrow>\amp = \lim\limits_{(x_0+iy)  \to (x_0+iy_0)}\frac{(x_0-iy) -(x_0-iy_0)}{(x_0-x_0) +i(y-y_0)}</mrow>
          <mrow>\amp = \lim\limits_{(x_0+iy)  \to (x_0+iy_0)}\frac{-i(y-y_0)}{i(y-y_0)}</mrow>
          <mrow>\amp = -1</mrow>
        </md>.
      </p>
      <p>
        The limits along the two paths are different,
        so there is no possible value for the right side of Equation <xref ref="Deriv_Def_1"/>.
        Therefore <m>f( z) = \overline{z}</m> is not differentiable at the point <m>z_0</m>,
        and since <m>z_0</m> was arbitrary,
        <m>f(z)</m> is nowhere differentiable.
      </p>
    </solution>
  </example>
  <remark>
    <p>
      In <xref ref="sec_limits-continuity">Section</xref>
      we showed that <m>f(z) = \overline{z}</m> is continuous for all <m>z</m>.
      Thus, we have a simple example of a function that is continuous everywhere but differentiable nowhere.
      Such functions are hard to construct in real variables.
      In some sense,
      the complex case has made pathological constructions simpler!
    </p>
  </remark>
  <p>
    We seldom are interested in studying functions that aren't differentiable,
    or are differentiable at only a single point.
    Complex functions that have a derivative at all points in a neighborhood of <m>z_0</m> deserve further study.
    In <xref ref="ch_taylor-laurent"/> we demonstrate that,
    if the complex function <m>f</m> can be represented by a Taylor series at <m>z_0</m>,
    then it must be differentiable in some neighborhood of <m>z_0</m>.
    Functions that are differentiable in neighborhoods of points are pillars of the complex analysis edifice;
    we give them a special name, as indicated in the following definition.
  </p>
  <definition xml:id="Analytic_Def">
    <title>Analytic</title>
    <statement>
      <p>
        The complex function <m>f</m> is
        <term>analytic at the point</term><m>z_0</m> provided there is some <m>\varepsilon>0</m> such that
        <m>f\,'( z)</m> exists for all <m>z\in D_{\varepsilon}(z_0)</m>.
        In other words,
        <m>f</m> must be differentiable not only at <m>z_0</m>,
        but also at all points in some
        <m>\varepsilon</m>-neighborhood of <m>z_0</m>.
      </p>
    </statement>
  </definition>
  <p>
    If <m>f</m> is analytic at each point in the region <m>R</m>,
    then we say that <m>f</m> is <term>analytic on</term><m>R</m>.
    Again, we have a special term if <m>f</m> is analytic on the whole complex plane.
  </p>
  <definition xml:id="Entire_Def">
    <title>Entire</title>
    <statement>
      <p>
        If <m>f</m> is analytic on the whole complex plane then <m>f</m> is said to be <term>entire</term>.
      </p>
    </statement>
  </definition>
  <p>
    Points of non analyticity for a function are called
    <term>singular points</term>.
    They are important for certain applications in physics and engineering.
  </p>
  <p>
    Our definition of the derivative for complex functions is formally the same as for real functions and is the natural extension from real variables to complex variables.
    The basic differentiation formulas are identical to those for real functions,
    and we obtain the same rules for differentiating powers, sums,
    products, quotients, and compositions of functions.
    We can easily establish the proof of the differentiation formulas by using the limit theorems.
  </p>
  <p>
    Suppose that <m>f</m> and <m>g</m> are differentiable.
    From Equation <xref ref="Deriv_Def_1"/> and the technique exhibited in the solution to <xref ref="DerivEx">Example</xref>,
    we can establish the following rules,
    which are virtually identical to those for real-valued functions.
    <md>
      <mrow xml:id="Deriv_Eq_4" number="yes">\frac{d}{dz}C \amp = 0,  \text{ where }   C  \text{ is a constant, and }</mrow>
      <mrow xml:id="Deriv_Eq_5" number="yes">\frac{d}{dz}z^{n} \amp = nz^{n-1},  \text{ where }   n  \text{ is a positive integer } .</mrow>
      <mrow xml:id="Deriv_Eq_6" number="yes">\frac{d}{dz}[Cf(z)] \amp = Cf\,'(z)</mrow>
      <mrow xml:id="Deriv_Eq_7" number="yes">\frac{d}{dz}[f(z)+g(z)] \amp = f\,'(z) + g\,'(z)</mrow>
      <mrow xml:id="Deriv_Eq_8" number="yes">\frac{d}{dz} [f(z) g(z)] \amp = f(z) g\,'(z) + g(z) f\,'(z)</mrow>
      <mrow xml:id="Deriv_Eq_9" number="yes">\frac{d}{dz}\frac{f(z)}{g(z)} \amp = \frac{g(z) f\,'(z) -f(z) g\,'(z)}{[g(z)]^2}  \text{ if } g(z) \ne 0,  \text{ and }</mrow>
      <mrow xml:id="Deriv_Eq_10" number="yes">\frac{d}{dz}\,f\big(g(z)\big) \amp = f\,'\big(g(z)\big) g\,'(z)</mrow>
    </md>.
  </p>
  <p>
    Important particular cases of Equations <xref ref="Deriv_Eq_9"/> and <xref ref="Deriv_Eq_10"/>, respectively, are
    <md>
      <mrow xml:id="Deriv_Eq_11" number="yes">\frac{d}{dz}\frac{1}{z^{n}} \amp = \frac{-n}{z^{n+1}}\text{ ,\qquad for } z \ne 0,  n  \text{ a positive integer, and }</mrow>
      <mrow xml:id="Deriv_Eq_12" number="yes">\frac{d}{dz}\left[ f(z) \right]^{n} \amp  =n\left[ f(z) \right]^{n-1}f\,'(z),  n  \text{ a positive integer. }</mrow>
    </md>
  </p>
  <example>
    <statement>
      <p>
        If we use Equation <xref ref="Deriv_Eq_12"/> with
        <m>f(z)=z^2+i2z+3</m> and <m>f\,'(z) =2z+2i</m>, then we get
        <me>
          \frac{d}{dz}(z^2+i2z+3)^{4}=8(z^2+i2z+3)^3(z+i)
        </me>.
      </p>
    </statement>
  </example>
  <p>
    The proofs of the rules given in Equations <xref ref="Deriv_Eq_4"/> through <xref ref="Deriv_Eq_10"/> depend on the validity of extending theorems for real functions to their complex companions.
    Equation <xref ref="Deriv_Eq_8"/>, for example, relies on Theorem 3.1.
  </p>
  <theorem xml:id="Diffl_Implies_Cont">
    <statement>
      <p>
        If <m>f</m> is differentiable at <m>z_0</m>,
        then <m>f</m> is continuous at <m>z_0</m>.
      </p>
    </statement>
  </theorem>
  <proof>
    <p>
      From Equation <xref ref="Deriv_Def_1"/>, we obtain
      <me>
        \lim_{z \to z_0}\frac{f(z) -f(z_0)}{z-z_0}=f\,'(z_0)
      </me>.
    </p>
    <p>
      Using the multiplicative property of limits given by <xref ref="limproduct">Formula</xref>, we get
      <md>
        <mrow>\lim\limits_{z \to z_0} [f(z) -f(z_0)] \amp = \lim_{z \to z_0}\frac{f(z) -f(z_0)}{z-z_0}(z-z_0)</mrow>
        <mrow>\amp = \lim_{z \to z_0}\frac{f(z) -f(z_0)}{z-z_0}\lim\limits_{z \to z_0}(z-z_0)</mrow>
        <mrow>\amp = f\,'(z_0) \cdot 0=0</mrow>
      </md>.
    </p>
    <p>
      This result implies that <m>\lim\limits_{z \to z_0}f(z) =f(z_0)</m>,
      which is equivalent to showing that <m>f</m> is continuous at <m>z_0</m>.
    </p>
  </proof>
  <p>
    We can establish Equation <xref ref="Deriv_Eq_8"/> from <xref ref="Diffl_Implies_Cont">Theorem</xref>.
    Letting <m>h(z)=f(z)g(z)</m> and using Definition 3.1, we write
    <me>
      h'(z_0) = \lim\limits_{z \to z_0}\frac{h(z) -h(z_0)}{z-z_0} = \lim_{z \to z_0}\frac{f(z) g(z)-f(z_0)g(z_0)}{z-z_0}
    </me>.
  </p>
  <p>
    If we subtract and add the term
    <m>f(z_0) g(z)</m> in the numerator, we get
    <md>
      <mrow>h'(z_0) \amp = \lim_{z \to z_0}\frac{f(z) g(z) - f(z_0) g(z) + f(z_0) g(z) - f(z_0)g(z_0)}{z-z_0}</mrow>
      <mrow>\amp = \lim_{z \to z_0}\frac{f(z)g(z) - f(z_0)g(z)}{z-z_0} + \lim_{z \to z_0}\frac{f(z_0)g(z) - f(z_0)g(z_0)}{z-z_0}</mrow>
      <mrow>\amp = \lim_{z \to z_0}\frac{f(z) -f(z_0)}{z-z_0}\lim_{z \to z_0}g(z) + f(z_0) \lim\limits_{z \to z_0}\frac{g(z) -g(z_0)}{z-z_0}</mrow>
    </md>.
  </p>
  <p>
    Using the definition of the derivative given by Equation <xref ref="Deriv_Def_1"/> and the continuity of <m>g</m>,
    we obtain <m>h'(z_0) =f\,'(z_0) g(z_0) +f(z_0) g\,'(z_0)</m>,
    which is what we wanted to establish.
    We leave the proofs of the other rules as exercises.
  </p>
  <p>
    The rule for differentiating polynomials carries over to the complex case as well.
    If we let <m>P(z)</m> be a polynomial of degree <m>n</m>, so
    <me>
      P(z)=a_0 + a_1z + a_2z^2 + \cdots + a_nz^n
    </me>.
    then mathematical induction,
    along with Equations <xref ref="Deriv_Eq_5"/> and <xref ref="Deriv_Eq_7"/>, gives
    <me>
      P\,'(z) =a_1 + 2a_2z + 3a_3z^2 + \cdots + na_nz^{n-1}
    </me>.
  </p>
  <p>
    Again, we leave the proof of this result as an exercise.
  </p>
  <p>
    We can use the differentiation rules as aids in determining when functions are analytic.
    For example, Equation <xref ref="Deriv_Eq_9"/> tells us that if <m>P(z)</m> and <m>Q(z)</m> are polynomials,
    then their quotient <m>\frac{P(z)}{Q(z)}</m> is analytic at all points where <m>Q(z) \ne 0</m>.
    This condition implies that the function
    <m>f(z) = \frac{1}{z}</m> is analytic for all <m>z\ne 0</m>.
    The square root function is more complicated.
    If <m>f(z)=z^{\frac{1}{2}} = |z|^{\frac{1}{2}}e^{i\frac{\mathrm{Arg}(z)}{2}}</m>,
    then <m>f</m> is analytic at all points except <m>z=0</m> (because
    <m>\mathrm{Arg}(0)</m> is undefined) and at points that lie along the negative <m>x</m> axis.
    The argument function, and therefore the function <m>f</m> itself,
    are not continuous at points that lie along the negative <m>x</m> axis.
  </p>
  <p>
    We close this section with a complex extension of a famous theorem,
    the proof of which will be given in <xref ref="ch_taylor-laurent"/>.
  </p>
  <theorem xml:id="LH_s_rule">
    <title>L'H&#xf4;pital's rule</title>
    <statement>
      <p>
        Assume that <m>f</m> and <m>g</m> are analytic at <m>z_0</m>.
        If <m>f(z_0) =0</m>, <m>g(z_0) =0</m>,
        and <m>g\,'(z_0) \ne 0</m>, then
        <me>
          \lim_{z \to z_0}\frac{f(z)}{g(z)} = \lim_{z \to z_0}\frac{f\,'(z)}{g\,'(z)}
        </me>.
      </p>
    </statement>
  </theorem>
  <proof>
    <p>
      See Corollary 7.11.
    </p>
  </proof>
  <exercises>
    <title>Exercises for <xref ref="sec_diff-analytic">Section</xref></title>
    <exercise xml:id="x3_1_1">
      <p>
        Find the derivatives of the following functions.
      </p>
      <ol>
        <li>
          <p>
            <m>g(z) =(z^2-iz+9)^{5}</m>.
          </p>
        </li>
        <li>
          <p>
            <m>h(z) = \frac{2z+1}{z+2}</m> for <m>z \ne -2</m>.
          </p>
        </li>
        <li>
          <p>
            <m>F(z) = (z^2+(1-3i)z+1)(z^4+3z^2+5i)</m>.
          </p>
        </li>
      </ol>
    </exercise>
    <exercise xml:id="x3_1_2">
      <p>
        Show that the following functions are differentiable nowhere.
        <ol>
          <li>
            <p>
              <m>f(z) = \mathrm{Re}(z)</m>.
            </p>
          </li>
          <li>
            <p>
              <m>f(z) = \mathrm{Im}(z)</m>.
            </p>
          </li>
        </ol>
      </p>
    </exercise>
    <exercise xml:id="x3_1_3">
      <p>
        If <m>f</m> and <m>g</m> are entire functions,
        which of the following are necessarily entire?
        <ol>
          <li>
            <p>
              <m>[f(z)]^3</m>.
            </p>
          </li>
          <li>
            <p>
              <m>f(z)g(z)</m>.
            </p>
          </li>
          <li>
            <p>
              <m>\frac{f(z)}{g(z)}</m>.
            </p>
          </li>
          <li>
            <p>
              <m>f(\frac{1}{z})</m>.
            </p>
          </li>
          <li>
            <p>
              <m>f(z-1)</m>.
            </p>
          </li>
          <li>
            <p>
              <m>f\big(g(z)\big)</m>.
            </p>
          </li>
        </ol>
      </p>
    </exercise>
    <exercise xml:id="x3_1_4">
      <p>
        Use Equation <xref ref="Deriv_Def_1"/> to verify <xref ref="Deriv_Eq_5">rule</xref>.
      </p>
    </exercise>
    <exercise xml:id="x3_1_5">
      <p>
        Let <m>P(z) =a_0+a_1z+\cdots +a_{n}z^{n}</m> be a polynomial of degree <m>n \ge 1</m>.
        <ol>
          <li>
            <p>
              Show that <m>P\,'(z) = a_1 + 2a_2z + \cdots + na_nz^{n-1}</m>.
            </p>
          </li>
          <li>
            <p>
              Show that, for <m>k=0,1, \ldots,
              n, \; a_{k}= \frac{P^{(k) }(0)}{k!}</m>,
              where <m>P^{(k)}</m> denotes the
              <m>k^{\text{ th } }</m> derivative of <m>P</m>. (By convention,
              <m>P^{(0)}(z) = P(z)</m>.)
            </p>
          </li>
        </ol>
      </p>
    </exercise>
    <exercise xml:id="x3_1_6">
      <p>
        Let <m>P</m> be a polynomial of degree 2, given by
        <me>
          P(z) = (z-z_1)(z-z_2)
        </me>.
        where <m>z_1\ne  z_2</m>.
        Show that
        <me>
          \frac{P\,'(z)}{P(z)} = \frac{1}{z-z_1} + \frac{1}{z-z_2}
        </me>.
        <em>Note</em>: The quotient <m>\frac{P\,'(z)}{P(z)}</m> is known as the
        <em>logarithmic derivative</em> of <m>P</m>.
      </p>
    </exercise>
    <exercise xml:id="x3_1_7">
      <p>
        Use L'H&#xf4;pital's rule to find the following limits.
        <ol>
          <li>
            <p>
              <m>\lim\limits_{z \to i}\frac{z^{4}-1}{z-i}</m>.
            </p>
          </li>
          <li>
            <p>
              <m>\lim\limits_{z \to 1+i}\frac{z^2-iz-1-i}{z^2-2z+2}</m>.
            </p>
          </li>
          <li>
            <p>
              <m>\lim\limits_{z \to -i}\frac{z^{6}+1}{z^2+1}</m>.
            </p>
          </li>
          <li>
            <p>
              <m>\lim\limits_{z \to 1+i}\frac{z^{4}+4}{z^2-2z+2}</m>.
            </p>
          </li>
          <li>
            <p>
              <m>\lim\limits_{z \to 1+i\sqrt{3}}\frac{z^{6}-64}{z^3+8}</m>.
            </p>
          </li>
          <li>
            <p>
              <m>\lim\limits_{z \to -1+i\sqrt{3}}\frac{z^{9}-512}{z^3-8}</m>.
            </p>
          </li>
        </ol>
      </p>
    </exercise>
    <exercise xml:id="x3_1_8">
      <p>
        Use Equation <xref ref="Deriv_Def_1"/> to show that <m>\frac{d}{dz}\frac{1}{z}= \frac{-1}{z^2}</m>.
      </p>
    </exercise>
    <exercise xml:id="x3_1_9">
      <p>
        Show that <m>\frac{d}{dz}z^{-n}=-nz^{-n-1}</m>,
        where <m>n</m> is a positive integer.
      </p>
    </exercise>
    <exercise xml:id="x3_1_10">
      <p>
        Verify the identity.
        <me>
          \frac{d}{dz} f(z)g(z)h(z) = f\,'(z)g(z)h(z) + f(z)g\,'(z)h(z) + f(z)g(z)h'(z)
        </me>.
      </p>
    </exercise>
    <exercise xml:id="x3_1_11">
      <p>
        Show that the function <m>f(z) =|z|^2</m> is differentiable only at the point <m>z_0=0</m>.
        <em>Hint</em>: To show that <m>f</m> is <em>not</em>
        differentiable at <m>z_0 \ne 0</m>,
        choose horizontal and vertical lines through the point <m>z_0</m> and show that
        <m>\frac{\Delta w}{ \Delta z}</m> approaches two distinct values as
        <m>\Delta z \to 0</m> along those two lines.
      </p>
    </exercise>
    <exercise>
      <p>
        Verify
        <ol>
          <li>
            <p>
              <xref ref="Deriv_Eq_4">Identity</xref>.
            </p>
          </li>
          <li>
            <p>
              <xref ref="Deriv_Eq_7">Identity</xref>.
            </p>
          </li>
          <li>
            <p>
              <xref ref="Deriv_Eq_9">Identity</xref>.
            </p>
          </li>
          <li>
            <p>
              <xref ref="Deriv_Eq_10">Identity</xref>.
            </p>
          </li>
          <li>
            <p>
              <xref ref="Deriv_Eq_12">Identity</xref>.
            </p>
          </li>
        </ol>
      </p>
    </exercise>
    <exercise xml:id="x3_1_13">
      <p>
        Consider the differentiable function
        <m>f(z)=z^3</m> and the two points <m>z_1=1</m> and <m>z_2=i</m>.
        Show that there does not exist a point <m>c</m> on the line <m>y=1-x</m> between 1 and <m>i</m> such that <m>\frac{f(z_2)-f(z_1)}{z_2-z_1} = f\,'(c)</m>.
        This result shows that the mean value theorem for derivatives does not extend to complex functions.
      </p>
    </exercise>
    <exercise xml:id="x3_1_14">
      <p>
        Let <m>f(z)=z^{\frac{1}{n}}</m> denote the multivalued
        <q><m>n</m>th root function,</q>
        where <m>n</m> is a positive integer.
        Use the chain rule to show that,
        if <m>g( z)</m> is any branch of the <m>n</m>th root function, then
        <me>
          g\,'(z) = \frac{1}{n}\frac{g(z)}{z}
        </me>
        in some suitably chosen domain
        (which you should specify).
      </p>
    </exercise>
    <exercise xml:id="x3_1_15">
      <p>
        Explain why the composition of two entire functions is an entire function.
      </p>
    </exercise>
    <exercise>
      <p>
        Let <m>f</m> be differentiable at <m>z_0</m>.
        Show that there exists a function <m>\eta(z)</m> such that
        <me>
          f(z) =f(z_0) +f\,'(z_0) (z-z_0) + \eta(z)(z-z_0)
        </me>,
        where <m>\eta (z)  \to 0\text{ as } z \to z_0</m>.
      </p>
    </exercise>
  </exercises>
</section>