<section xml:id="sec_exponential-function">
  <title>The Complex Exponential Function</title>
  <p>
    Recall that the real exponential function can be represented by the power series <m>e^x=\sum\limits_{n=0}^{\infty }\frac{1}{n!}x^n</m>.
    Thus it is only natural to define the complex exponential <m>e^z</m>,
    also written as <m>\exp(z)</m>,in the following way.
  </p>
  <definition xml:id="exp_z__Def">
    <title>The Complex Exponential</title>
    <statement>
      <me>
        e^z=\exp(z) =\sum_{n=0}^{\infty }\frac{1}{n!}z^n
      </me>.
    </statement>
  </definition>
  <p>
    Clearly, this definition agrees with that of the real exponential function when <m>z</m> is a real number.
    We now show that this complex exponential has two of the key properties associated with its real counterpart and verify the identity <m>e^{i\theta }=\cos \theta +i\sin \theta</m>, which,
    back in <xref ref="ch_Complex_Numbers"/>
    (see <xref ref="Euler_s_Formula">Identity</xref>
    of <xref ref="sec_geometry-2">Section</xref>)
    we promised to establish.
  </p>
  <theorem xml:id="thm_exp_properties">
    <statement>
      <p>
        The function <m>\exp z</m> is an entire function satisfying the following conditions.
        <ol>
          <li>
            <title>i</title>
            <p>
              <m>\exp^{\,\prime}(z)=\exp(z)=e^z</m>
              (using the Leibniz notation, <m>\frac{d}{dz}e^z=e^z</m>).
            </p>
          </li>
          <li>
            <title>ii</title>
            <p>
              <m>\exp(z_1+z_2) =\exp(z_1) \exp(z_2)</m>
              (<em>i.e.</em>, <m>e^{z_1+z_2}=e^{z_1}e^{z_2}</m>).
            </p>
          </li>
          <li>
            <title>iii</title>
            <p>
              If <m>\theta</m> is a real number,
              then <m>e^{i\theta }=\cos \theta +i\sin \theta</m>.
            </p>
          </li>
        </ol>
      </p>
    </statement>
  </theorem>
  <proof>
    <p>
      By the ratio test
      (check Example 4.23),
      the series in Definition 5.1 has an infinite radius of convergence,
      so <m>\exp(z)</m> is entire by <xref ref="Power_Series_Thm">Theorem</xref>,
      part (i).
    </p>
    <p>
      Using <xref ref="Power_Series_Thm">Theorem</xref>, part (ii), we get
      <me>
        \exp^{\,\prime }(z) =\sum\limits_{n=1}^{\infty }\frac{n}{n!} z^{n-1}= \sum\limits_{n=1}^{\infty }\frac{1}{(n-1)!}z^{n-1} = \sum\limits_{n=0}^{\infty }\frac{1}{n!}z^n=\exp(z)
      </me>,
      which gives us part (i) of <xref ref="thm_exp_properties">Theorem</xref>
    </p>
    <p>
      To prove part (ii),
      we let <m>\zeta</m> be an arbitrary complex number and define <m>g(z)</m> to be
      <me>
        g(z)=\exp(z)\exp(\zeta -z)
      </me>.
    </p>
    <p>
      Using the product rule, chain rule, and part (i), we have
      <me>
        g^{\,\prime }(z) =\exp(z) \exp(\zeta -z) + \exp(z)[-\exp(\zeta -z)] =0 \text{ for all } z
      </me>.
    </p>
    <p>
      According to Theorem 4.16,
      this result implies that the function <m>g</m> must be constant.
      Thus, for all <m>z</m>, <m>g(z)=g(0)</m>.
      Since <m>\exp()=1</m> (verify!), we deduce
      <me>
        g(z) =g(0) =\exp(0) \exp(\zeta -0)=\exp(\zeta)
      </me>.
    </p>
    <p>
      Hence, for all <m>z</m>,
      <me>
        g(z)=\exp(z) \exp(\zeta -z)=\exp(\zeta)
      </me>.
    </p>
    <p>
      Setting <m>z=z_1</m> and letting <m>\zeta =z_1+z_2</m>, we get
      <me>
        \exp(z_1) \exp(z_1+z_2-z_1) =\exp(z_1+z_2)
      </me>,
      which simplifies to our desired result.
    </p>
    <p>
      To prove part (iii), we let <m>\theta</m> be a real number.
      By Definition 5.1,
      <md>
        <mrow>e^{i\theta } \amp = \exp(i\theta )</mrow>
        <mrow>\amp = \sum_{n=0}^{\infty}\frac{1}{n!}(i\theta)^n</mrow>
        <mrow>\amp = \sum_{n=0}^{\infty }\left[\frac{1}{( 2n)!} (i\theta)^{2n}+\frac{1}{( 2n+1)!}( i\theta)^{2n+1}\right] {\text{ (separating odd and even exponents) } }</mrow>
        <mrow>\amp = \sum_{n=0}^{\infty }\left[\frac{1}{(2n)!}(i^2)^n\theta^{2n} + \frac{1}{(2n+1)!}i(i^2 )^n\theta^{2n+1}\right]</mrow>
        <mrow>\amp = \sum_{n=0}^{\infty}(-1)^n \frac{\theta^{2n}}{(2n)!} + i\sum_{n=0}^{\infty}(-1)^n\frac{\theta^{2n+1}}{(2n+1)!}</mrow>
        <mrow>\amp = \cos \theta +i\sin \theta  {\text{ (by the series representations for the real-valued sine and cosine) } }</mrow>
      </md>.
    </p>
  </proof>
  <p>
    Note that parts (ii) and (iii) of the <xref ref="thm_exp_properties">Theorem</xref>
    combine to verify DeMoivre's formula,
    which we introduced in <xref ref="sec_algebra-2">Section</xref>
    (see <xref ref="De_Moivre_s_formula">Identity</xref>).
  </p>
  <p>
    If <m>z=x+iy</m>, then from parts (ii) and (iii) we have
    <men xml:id="e_z_Cartesian">
      \exp(z) = e^z = e^{x+iy} = e^xe^{iy} = e^x(\cos y+i\sin y)
    </men>.
  </p>
  <p>
    Some texts start with <xref ref="e_z_Cartesian">Identity</xref>
    as the definition for <m>\exp(z)</m>.
    In the exercises,
    we show that this is a natural approach from the standpoint of differential equations.
  </p>
  <p>
    The notation <m>\exp(z)</m> is preferred over <m>e^z</m> in some situations.
    For example,
    <m>\exp(\frac{{1}}{5}) =1.22140275816017\ldots</m> is the value of <m>\exp(z)</m> when
    <m>z=\frac{{1}}{5}</m> and equals the positive fifth root of <m>e=2.71828182845904\ldots </m>.
    Thus, the notation <m>e^{\frac{{1}}{5}}</m> is ambiguous and might be interpreted as any of the complex fifth roots of the number <m>e</m> that we discussed in <xref ref="sec_algebra-2">Section</xref>:
    <me>
      e^{\frac{{1}}{5}}\approx 1.22140275816017\left(\cos \frac{2\pi k}{5}+ i\sin\frac{2\pi k}{5}\right), \text{ for }   k=0,\,1, \, \ldots, \,4
    </me>.
  </p>
  <p>
    To prevent this confusion,
    we often use <m>\exp(z)</m> to denote the single-valued exponential function.
  </p>
  <p>
    We now explore some additional properties of <m>\exp(z)</m>.
    Using <xref ref="e_z_Cartesian">Identity</xref>,
    we can easily establish that
    <md>
      <mrow xml:id="e_z_Periodic" number="yes">e^{z+i2n\pi} \amp =e^z, \amp \amp  \text{ for all } z\text{ , provided } n\text{ is an integer } ,</mrow>
      <mrow xml:id="e_z___1" number="yes">e^z \amp =1, \amp \amp  \text{ iff } z=i2n\pi \text{ , where } n\text{ is an integer, and }</mrow>
      <mrow xml:id="e_z1___e_z2" number="yes">e^{z_1} \amp =e^{z_2}, \amp \amp  \text{ iff } z_2=z_1+i2n\pi \text{ for some integer } n</mrow>
    </md>.
  </p>
  <p>
    For example, because <xref ref="e_z_Cartesian">Identity</xref>
    involves the periodic functions <m>\cos y</m> and <m>\sin y</m>,
    any two points in the <m>z</m> plane that lie on the same vertical line with their imaginary parts differing by an integral multiple of <m>2\pi</m> are mapped onto the same point in the <m>w</m> plane.
    Thus the complex exponential function is periodic with period <m>2\pi i</m>,
    which establishes Equation <xref ref="e_z_Periodic"/>.
    We leave the verification of Equations <xref ref="e_z___1"/> and <xref ref="e_z1___e_z2"/> as exercises.
  </p>
  <example xml:id="ex_exp_mapping">
    <statement>
      <p>
        For any integer <m>n</m>, the points
        <me>
          z_n=\frac{5}{4}+i\left(\frac{11\pi }{6}+2n\pi\right)
        </me>
        in the <m>z</m> plane are mapped onto the single point
        <me>
          w_{0}  = \exp(z_n) = e^{\frac{5}{4}}\left(\cos \frac{11\pi }{6}+i\sin \frac{11\pi }{6}\right) = \frac{\sqrt{3}}{2}e^{\frac{5}{4}}-i\frac{1}{2}e^{\frac{5}{4}} \approx 3.02-1.75i
        </me>
        in the <m>w</m> plane,
        as indicated in <xref ref="fig_ch-05-01">Figure</xref>.
      </p>
    </statement>
  </example>
  <figure xml:id="fig_ch-05-01">
    <caption>The points <m>\{z_n\}</m> in the <m>z</m> plane (<em>i.e.</em>, the <m>xy</m> plane) and their image <m>w_{0}=\exp(z_n)</m> in the <m>w</m> plane
    (<em>i.e.</em>, the <m>uv</m> plane)</caption>
    <image width="73%" source="figs/ch-05/ch-05-fig-01.pdf"/>
  </figure>
  <p>
    Let's look at the range of the exponential function.
    If <m>z=x+iy</m>,
    we see from <xref ref="e_z_Cartesian">Identity</xref><mdash/><m>e^z=e^xe^{iy}=e^x( \cos y+i\sin y)</m><mdash/>that <m>e^z</m> can never equal zero,
    as <m>e^x</m> is never zero,
    and the cosine and sine functions are never zero at the same point.
    Suppose, then, that <m>w=e^z \ne 0</m>.
    If we write <m>w</m> in its exponential form as <m>w=\rho e^{i\phi }</m>,
    <xref ref="e_z_Cartesian">Identity</xref> gives
    <me>
      \rho e^{i\phi }=e^xe^{iy}
    </me>.
  </p>
  <p>
    Using <xref ref="e_z_Cartesian">Identity</xref>,
    and <xref ref="ExpEquality">Property</xref>
    of <xref ref="sec_algebra-2">Section</xref>, we get
    <md>
      <mrow xml:id="rho_and_phi" number="yes">\rho \amp =\amp e^x\text{ and } \phi =y+2n\pi \text{ , where } n\text{ is an integer. Therefore, }</mrow>
      <mrow xml:id="abs_rho" number="yes">\rho \amp =\amp |e^z| =e^x,\text{ and }</mrow>
      <mrow xml:id="phi" number="yes">\phi \amp \in \amp \arg(e^z) =\{\mathrm{Arg}( e^z) +2n\pi :n\text{ is an integer } \}</mrow>
    </md>.
  </p>
  <p>
    Solving Equations <xref ref="rho_and_phi"/> for <m>x</m> and <m>y</m> yields
    <men xml:id="Inverse_of_Exp">
      x=\ln \rho \ \ \text{ and } y=\phi +2n\pi
    </men>,
    where <m>n</m> is an integer.
    Thus for any complex number <m>w \ne 0</m>,
    there are infinitely many complex numbers <m>z=x+iy</m> such that <m>w=e^z</m>.
    From Equations <xref ref="Inverse_of_Exp"/>, the numbers <m>z</m> are
    <md>
      <mrow>z \amp = x+iy=\ln \rho +i( \phi +2n\pi )</mrow>
      <mrow xml:id="Inverse_of_Exp_again" number="yes">\amp = \ln |w| +i( \mathrm{Arg}\textit{ }w+2n\pi )</mrow>
    </md>.
    where <m>n</m> is an integer.
    Hence
    <me>
      \exp\big[|w| +i(\mathrm{Arg}\,w+2n\pi)\big] = w
    </me>.
  </p>
  <p>
    In summary, the transformation <m>w=e^z</m> maps the complex plane
    (infinitely often)
    onto the set of nonzero complex numbers.
  </p>
  <p>
    If we restrict the solutions to Equation <xref ref="Inverse_of_Exp_again"/> so that only the principal value of the argument,
    <m>-\pi \lt \mathrm{Arg}\,w \le \pi</m>, is used,
    the transformation <m>w=e^z=e^{x+iy}</m> maps the horizontal strip
    <m>\{(x,y):-\pi \lt y \le \pi \}</m> one-to-one and onto the range set <m>S=\{w:w \ne 0\}</m>.
    This strip is called the <term>fundamental period strip</term>
    and is shown in <xref ref="fig_ch-05-02">Figure</xref>.
  </p>
  <figure xml:id="fig_ch-05-02">
    <caption>The fundamental period strip for the mapping <m>w=\exp(z)</m></caption>
    <image width="73%" source="figs/ch-05/ch-05-fig-02.pdf"/>
  </figure>
  <p>
    The horizontal line <m>z=t+ib</m>,
    for <m>-\infty \lt t\lt \infty</m> in the <m>z</m> plane,
    is mapped onto the ray <m>w=e^{t}e^{ib}=e^{t}( \cos b+i\sin b)</m> that is inclined at an angle <m>\phi =b</m> in the <m>w</m> plane.
    The vertical segment <m>z=a+i\theta</m>,
    for <m>-\pi \lt \theta \le \pi</m> in the <m>z</m> plane,
    is mapped onto the circle centered at the origin with radius <m>e^{a}</m> in the <m>w</m> plane.
    That is, <m>w=e^{a}e^{i\theta }=e^{a}( \cos \theta +i\sin \theta )</m>.
    The lines <m>r_1</m>, <m>r_2</m>,
    and <m>r_3</m>, are mapped to the rays <m>r_1^{\ast}</m>,
    <m>r_2^{\ast}</m>, and <m>r_3^{\ast}</m>, respectively.
    Likewise, the segments <m>s_1</m>, <m>s_2</m>,
    and <m>s_3</m> are mapped to the corresponding circles <m>s_1^{\ast}</m>,
    <m>s_2^{\ast}</m>, and <m>s_3^{\ast}</m>.
  </p>
  <example xml:id="Rectangle_Map">
    <statement>
      <p>
        Consider a rectangle <m>R=\{(x,y) : a \le x \le b\text{ and } c \le y \le d\}</m>,
        where <m>-\pi \lt c\lt d \le \pi</m>.
        Show that the transformation
        <m>w=e^z=e^{x+iy}</m> maps <m>R</m> onto a portion of an annular region bounded by two rays.
      </p>
    </statement>
    <solution>
      <p>
        The image points in the <m>w</m> plane satisfy the following relationships involving the modulus and argument of <m>w</m>:
        <md>
          <mrow>e^{a}  \amp = |e^{a+iy}|  \le |e^{x+iy}| \le |e^{b+iy}| = e^b,  \text{ and }</mrow>
          <mrow>c     \amp = \mathrm{Arg}( e^{x+ic})  \le \mathrm{Arg}(e^{x+iy}) \le \mathrm{Arg}( e^{x+id}) \le d</mrow>
        </md>.
        which is a portion of the annulus
        <m>\{\rho e^{i\phi }:e^a \le \rho \le e^b\}</m> in the <m>w</m> plane subtended by the rays <m>\phi =c</m> and <m>\phi =d</m>.
        In <xref ref="fig_ch-05-03">Figure</xref>,
        we show the image of the rectangle
        <me>
          R = \left\{(x,y) :-1 \le x \le 1\text{ and } \frac{-\pi }{4} \le y \le \frac{\pi }{3}\right\}
        </me>.
      </p>
    </solution>
  </example>
  <figure xml:id="fig_ch-05-03">
    <caption>The image of <m>R</m> under the transformation <m>w=\exp(z)</m></caption>
    <image width="73%" source="figs/ch-05/ch-05-fig-03.pdf"/>
  </figure>
  <exercises>
    <title>Exercises for <xref ref="sec_exponential-function">Section</xref></title>
    <exercise xml:id="x5_1_1">
      <p>
        Using Definition 5.1, explain why <m>\exp (0) =e^{0}=1</m>.
      </p>
    </exercise>
    <exercise xml:id="x5_1_2">
      <p>
        The questions for this problem relate to Figure 5.2.
        The shaded portion in the <m>w</m> plane indicates the image of the shaded portion in the <m>z</m> plane,
        with the lighter shading indicating expansion of the area of corresponding regions.
      </p>
      <ol>
        <li>
          <p>
            Why is there no shading inside the circle <m>s_1^{\ast}</m>?
          </p>
        </li>
        <li>
          <p>
            Explain why the images of <m>r_1</m>,
            <m>r_2</m>, and <m>r_3</m> appear to make,
            respectively,
            angles of <m>-\frac{7\pi }{8}</m>, <m>\frac{\pi}{4}</m>,
            and <m>\frac{3\pi}{4}</m> radians with the positive <m>u</m> axis.
          </p>
        </li>
        <li>
          <p>
            Precisely where should the images of the points <m>\pm i\pi</m> be located?
          </p>
        </li>
      </ol>
    </exercise>
    <exercise xml:id="x5_1_3">
      <p>
        Verify Equations <xref ref="e_z___1"/> and <xref ref="e_z1___e_z2"/>.
      </p>
    </exercise>
    <exercise xml:id="x5_1_4">
      <p>
        Express <m>e^z</m> in the form <m>u+iv</m> for the following values of <m>z</m>.
        <ol>
          <li>
            <p>
              <m>\frac{-\pi }{3}</m>.
            </p>
          </li>
          <li>
            <p>
              <m>\frac{1}{2}-i\frac{\pi }{4}</m>.
            </p>
          </li>
          <li>
            <p>
              <m>-4+5i</m>.
            </p>
          </li>
          <li>
            <p>
              <m>-1+i\frac{3\pi }{2}</m>.
            </p>
          </li>
          <li>
            <p>
              <m>1+i\frac{5\pi }{4}</m>.
            </p>
          </li>
          <li>
            <p>
              <m>\frac{\pi }{3}-2i</m>.
            </p>
          </li>
        </ol>
      </p>
    </exercise>
    <exercise>
      <p>
        Find all values of <m>z</m> for which the following equations hold.\label {5.1.5}
        <ol>
          <li>
            <p>
              <m>e^z=-4</m>.
            </p>
          </li>
          <li>
            <p>
              <m>e^z=2+2i</m>.
            </p>
          </li>
          <li>
            <p>
              <m>e^z=\sqrt{3}-i</m>.
            </p>
          </li>
          <li>
            <p>
              <m>e^z=-1+i\sqrt{3}</m>.
            </p>
          </li>
        </ol>
      </p>
    </exercise>
    <exercise xml:id="x5_1_6">
      <p>
        Prove that <m>|\exp(z^2 )| \le \exp\big(|z|^2\big)</m> for all <m>z</m>.
        Where does equality hold?
      </p>
    </exercise>
    <exercise xml:id="x5_1_7">
      <p>
        Show that <m>\exp(z+i\pi ) =\exp(z-i\pi )</m> holds for all <m>z</m>.
      </p>
    </exercise>
    <exercise xml:id="x5_1_8">
      <p>
        Express <m>\exp(z^2 )</m> and
        <m>\exp\left(\frac{1}{z}\right)</m> in the Cartesian form <m>u( x,y) +iv( x,y)</m>.
      </p>
    </exercise>
    <exercise xml:id="x5_1_9">
      <p>
        Explain why
        <ol>
          <li xml:id="x5_1_9a">
            <p>
              <m>\exp(\overline{z}) = \overline{\exp z}</m> holds for all <m>z</m>.
            </p>
          </li>
          <li xml:id="x5_1_9b">
            <p>
              <m>\exp(\overline{z})</m> is nowhere analytic.
            </p>
          </li>
        </ol>
      </p>
    </exercise>
    <exercise xml:id="x5_1_10">
      <p>
        Show that <m>|e^{-z}| \lt 1</m> iff <m>\mathrm{Re}(z) >0</m>.
      </p>
    </exercise>
    <exercise>
      <p>
        Verify that
        <ol>
          <li>
            <p>
              <m>\lim\limits_{z \to 0}\frac{e^z-1}{z}=1</m>.
            </p>
          </li>
          <li>
            <p>
              <m>\lim\limits_{z \to i\pi}\frac{e^z+1}{z-i\pi } = -1</m>.
            </p>
          </li>
        </ol>
      </p>
    </exercise>
    <exercise xml:id="x5_1_12">
      <p>
        Show that <m>f(z)=ze^z</m> is analytic for all <m>z</m> by showing that its real and imaginary parts satisfy the Cauchy-Riemann sufficient conditions for differentiability.
      </p>
    </exercise>
    <exercise>
      <p>
        Find the derivatives of the following.
        <ol>
          <li>
            <p>
              <m>e^{iz}</m>.
            </p>
          </li>
          <li>
            <p>
              <m>z^4\exp(z^3)</m>.
            </p>
          </li>
          <li>
            <p>
              <m>e^{(a+ib)z}</m>.
            </p>
          </li>
          <li>
            <p>
              <m>\exp(\frac{1}{z})</m>.
            </p>
          </li>
        </ol>
      </p>
    </exercise>
    <exercise xml:id="x5_1_14">
      <p>
        Let <m>n</m> be a positive integer.
        Show that
        <ol>
          <li>
            <p>
              <m>(\exp z)^n = \exp(nz)</m>.
            </p>
          </li>
          <li>
            <p>
              <m>\frac{1}{(\exp z)^n} = \exp(-nz)</m>.
            </p>
          </li>
        </ol>
      </p>
    </exercise>
    <exercise xml:id="x5_1_15">
      <p>
        Show that <m>\sum\limits_{n=0}^{\infty}e^{inz}</m> converges for <m>\mathrm{Im}(z)>0</m>.
      </p>
    </exercise>
    <exercise xml:id="x5_1_16">
      <p>
        Generalize <xref ref="ex_exp_mapping">Example</xref>,
        where the condition <m>-\pi \lt c\lt d \le \pi</m> is replaced by <m>d-c\lt 2\pi</m>.
        Illustrate what this means.
      </p>
    </exercise>
    <exercise xml:id="x5_1_17">
      <p>
        Use the fact that <m>\exp(z^2)</m> is analytic to show that
        <m>e^{x^2-y^2}\sin 2xy</m> is a harmonic function.
      </p>
    </exercise>
    <exercise xml:id="x5_1_18">
      <p>
        Show the following concerning the exponential map.
        <ol>
          <li>
            <p>
              The image of the line <m>\{(x,y) :x=t, \; y=2\pi+t\}</m>,
              where <m>-\infty \lt t\lt \infty</m> is a spiral.
            </p>
          </li>
          <li>
            <p>
              The image of the first quadrant<m>\{(x,y):x>0, \; y>0\}</m> is the region <m>\{w:|w| > 1\}</m>.
            </p>
          </li>
          <li>
            <p>
              If <m>a</m> is a real constant,
              the horizontal strip <m>\{(x,y) :\alpha \lt y \le \alpha +2\pi \}</m> is mapped one-to-one and onto the nonzero complex numbers.
            </p>
          </li>
          <li>
            <p>
              The image of the vertical line segment
              <m>\{(x,y):
              x=2, \; y=t\}</m>,
              where <m>\frac{\pi }{6} \lt t \lt \frac{7\pi }{6}</m> is half a circle.
            </p>
          </li>
          <li>
            <p>
              The image of the horizontal ray <m>\{(x,y) :x>0, \; y= \frac{\pi }{3}\}</m> is a ray.
            </p>
          </li>
        </ol>
      </p>
    </exercise>
    <exercise xml:id="x5_1_19">
      <p>
        Explain how the complex function <m>e^z</m> and the real function <m>e^x</m> are different.
        How are they similar?
      </p>
    </exercise>
    <exercise xml:id="x5_1_20">
      <p>
        Many texts give an alternative definition for <m>\exp(z)</m>,
        starting with Identity <xref ref="e_z_Cartesian"></xref>
        as the definition for <m>f(z)=\exp(z)</m>.
        Recall that this identity states that <m>\exp(z)=\exp(x+iy)=e^x( \cos y+i\sin y)</m>.
        This exercise shows such a definition is a natural approach in terms of differential equations.
        We start by requiring <m>f(z)</m> to be the solution to an initial-value problem satisfying three conditions: (1) <m>f</m> is entire, (2)
        <m>f\,'(z)=f(z)</m> for all <m>z</m>, and (3) <m>f(0)=1</m>.
        Suppose that <m>f(z)=f( x+iy)=u( x,y)+iv( x,y)</m> satisfies conditions (1), (2), and (3).
        <ol>
          <li>
            <p>
              Use the result <m>f\,'(z) =u_{x}(x,y)+iv_{x}( x,y)</m> and the requirement
              <m>f\,'(z)=f(z)</m> from condition (2) to show that
              <m>u_x(x,y) - u(x,y)=0</m>, for all <m>z=(x,y)</m>.
            </p>
          </li>
          <li>
            <p>
              Show that the result in part (a) implies that <m>\frac{\partial }{\partial x}[u(x,y) e^{-x}] =0</m>.
              This means <m>u(x,y)e^{-x}</m> is constant with respect to <m>x</m>,
              so <m>u(x,y)e^{-x}=p(y)</m>, where <m>p(y)</m> is a function of <m>y</m> alone.
            </p>
          </li>
          <li>
            <p>
              Using a similar procedure for <m>v(x,y)</m>,
              show we wind up getting a pair of solutions <m>u(x,y)=p(y)e^x</m>,
              and <m>v(x,y)=q(y)e^x</m> where <m>p(y)</m> and <m>q(y)</m> are functions of <m>y</m> alone.
            </p>
          </li>
          <li>
            <p>
              Now use the Cauchy-Riemann equations to conclude from part (c) that
              <m>p(y) =q^{\,\prime }(y)</m> and <m>p^{\,\prime }(y)=-q(y)</m>.
            </p>
          </li>
          <li>
            <p>
              Use part (d) to show that <m>p^{\,\prime \prime }(y) +p(y) =0</m> and <m>q^{\,\prime \prime }(y)+q(y)=0</m>.
            </p>
          </li>
          <li>
            <p>
              Identify the general solutions to part (e).
              Then, given the initial conditions <m>f(0) =f(0+0i)=u(0,0)+iv(0,0)=1+0i</m>,
              find the particular solutions and conclude that <xref ref="e_z_Cartesian">Identity</xref> follows.
            </p>
          </li>
        </ol>
      </p>
    </exercise>
  </exercises>
</section>