<section xml:id="sec_shifting-thms">
  <title>Shifting Theorems and the Step Function</title>
  <p>
    We have seen how the Laplace transform can be used to solve linear differential equations.
    Familiar functions that arise in solutions to differential equations are
    <m>e^{at}\cos bt</m> and <m>e^{at}\sin bt</m>.
    The <em>first shifting theorem</em>
    will show how their transforms are related to those of <m>\cos bt</m> and <m>\sin bt</m> by shifting the variable <m>s</m> in <m>F(s)</m>.
    A companion result, called the <em>second shifting theorem,</em>
    will show how the transform of <m>f(t-a)</m> can be obtained by multiplying <m>F(s)</m> by <m>e^{-as}</m>.
    Loosely speaking,
    these results show that multiplication of <m>f(t)</m> by <m>e^{at}</m> corresponds to shifting <m>F(s-a)</m>,
    and shifting <m>f( t-a)</m> corresponds to multiplication of the transform <m>F( s)</m> by <m>e^{as}</m>.
  </p>
  <theorem xml:id="thm_shifting-s">
    <title>Shifting the Variable
    <q>$s$</q>
    </title>
    <statement>
      <p>
        If <m>F(s)</m> is the Laplace transform of <m>f(t)</m>, then
        <me>
          \mathcal{L}\big(e^{at}f(t)\big) = F(s-a)
        </me>.
      </p>
    </statement>
  </theorem>
  <proof>
    <p>
      Using the integral definition <m>\mathcal{L}\big(f(t)\big) = F(s) = \int_0^{\infty}f(t)e^{-st}\,dt</m>,
      we see that
      <me>
        \mathcal{L}(e^{at}f(t)) = \int_0^{\infty}e^{at}f(t)e^{-st}dt = \int_0^{\infty}f(t)e^{-(s-a)t}\,dt = F(s-a)
      </me>.
    </p>
  </proof>
  <definition xml:id="def_unit-step-function">
    <title>Unit Step Function</title>
    <statement>
      <p>
        For <m>a \ge 0</m> the unit step function <m>U_a(t)</m> is
        <me>
          U_a(t) = \begin{cases}0 \amp  \text{ for }    t\lt a. \\ 1 \amp  \text{ for }    t>a. \end{cases}
        </me>
      </p>
    </statement>
  </definition>
  <p>
    <xref ref="fig_ch-11-22">Figure</xref>
    depicts the graph of <m>U_a(t)</m>.
  </p>
  <figure xml:id="fig_ch-11-22">
    <caption>Graph of the unit step function <m>y=U_a(t)</m> in <xref ref="def_unit-step-function">Definition</xref></caption>
    <image width="73%" source="figs/ch-11/ch-11-fig-22.pdf"/>
  </figure>
  <theorem xml:id="thm_shifting-t">
    <title>Shifting the Variable
    <q>$t$</q>
    </title>
    <statement>
      <p>
        If <m>F(s)</m> is the Laplace transform of <m>f(t)</m> and <m>a \ge 0</m>, then
        <me>
          \mathcal{L}\big(U_a(t)f(t-a)\big) = e^{-as}F(s)
        </me>,
        where <m>f(t)</m> and <m>U_a(t)(t-a)</m> are illustrated in <xref ref="fig_ch-11-23">Figure</xref>.
      </p>
    </statement>
  </theorem>
  <proof>
    <p>
      Using the definition of Laplace transform, we write
      <me>
        e^{-as}F(s) = e^{-as}\int_0^{\infty}f(\tau)e^{-s\tau}\,d\tau = \int_0^{\infty}f(\tau)e^{-s(a+\tau)}\,d\tau
      </me>.
    </p>
    <p>
      Using the change of variable
      <m>t=a+\tau</m> and <m>dt=d\tau</m>, we obtain
      <me>
        e^{-as}F(s) = \int_a^{\infty}f(t-a)e^{-st}\,dt
      </me>.
    </p>
    <p>
      Since <m>U_a(t) \,f(t-a) =0</m> for <m>t\lt a</m>,
      and <m>U_a(t) \,f(t-a) =f(t-a)</m> for <m>t>a</m>,
      we can write the last equation as
      <me>
        e^{-as}F(s) = \int_0^{\infty}U_a(t)f(t-a)e^{-st}\,dt = \mathcal{L}\big(U_a(t)f(t-a)\big)
      </me>.
    </p>
  </proof>
  <figure xml:id="fig_ch-11-23">
    <caption>Comparison of the functions <m>f(t)</m> and <m>U_a(t)f(t-a)</m></caption>
    <image width="73%" source="figs/ch-11/ch-11-fig-23.pdf"/>
  </figure>
  <example>
    <statement>
      <p>
        Show that <m>\mathcal{L}(t^ne^{at}) =\frac{n!}{(s-a)^{n+1}}</m>.
      </p>
    </statement>
    <solution>
      <p>
        Let <m>f(t)=t^n</m>,
        then <m>F(s) = \mathcal{L}(t^n) = \frac{n!}{s^{n+1}}</m>.
        Applying <xref ref="thm_shifting-s">Theorem</xref>,
        we obtain the desired result:
        <me>
          \mathcal{L}(t^ne^{at}) = F(s-a) = \frac{n!}{(s-a)^{n+1}}
        </me>.
      </p>
    </solution>
  </example>
  <example xml:id="ex_10_18">
    <statement>
      <p>
        Show that <m>\mathcal{L}(U_c(t)) = \frac{e^{-cs}}{s}</m>.
      </p>
    </statement>
    <solution>
      <p>
        Set <m>f(t) = 1</m>, then <m>F(s) = \mathcal{L}(1) = \frac{1}{s}</m>.
        Now apply <xref ref="thm_shifting-t">Theorem</xref> and get
        <me>
          \mathcal{L}\big(U_c(t)\big) = \mathcal{L}\big(U_c(t)f(t)\big) = \mathcal{L}\big(U_c(t)\cdot 1\big) = e^{-cs}\mathcal{L}(1) = \frac{e^{-cs}}{s}
        </me>.
      </p>
    </solution>
  </example>
  <example xml:id="ex_find-Lft">
    <statement>
      <p>
        Find <m>\mathcal{L}\big(f(t)\big)</m> if <m>f(t)</m> is given in <xref ref="fig_ch-11-24">Figure</xref>.
      </p>
      <figure xml:id="fig_ch-11-24">
        <caption>The function <m>y=f(t)</m> of <xref ref="ex_find-Lft">Example</xref></caption>
        <image width="73%" source="figs/ch-11/ch-11-fig-24.pdf"/>
      </figure>
    </statement>
    <solution>
      <p>
        We can represent <m>f(t)</m> in terms of step functions:
        <me>
          f(t) = 1-U_1(t)+U_2(t)-U_3(t)+U_4(t)-U_5(t)
        </me>.
      </p>
      <p>
        Using the result of <xref ref="ex_10_18">Example</xref> and linearity,
        we obtain
        <me>
          \mathcal{L}\big(f(t)\big) = \frac{1}{s} - \frac{e^{-s}}{s} + \frac{e^{-2s}}{s} - \frac{e^{-3s}}{s} + \frac{e^{-4s}}{s} - \frac{e^{-5s}}{s}
        </me>.
      </p>
    </solution>
  </example>
  <example>
    <statement>
      <p>
        Use Laplace transforms to solve the initial value problem
        <me>
          y^{\prime \prime}(t) + y(t) = U_{\pi}(t)  \text{ with }   y(0)=0  \text{ and }   y'(0) =0
        </me>.
      </p>
    </statement>
    <solution>
      <p>
        As usual, let <m>Y(s)</m> denote the Laplace transform of <m>y(t)</m>.
        Then we get
        <me>
          s^2Y(s) + Y(s) = \frac{e^{-\pi s}}{s}
        </me>.
      </p>
      <p>
        Solving for <m>Y(s)</m>, we obtain
        <me>
          Y(s) = e^{-\pi s}\frac{1}{s(s^2+1)} = \frac{e^{-\pi s}}{s} - \frac{e^{-\pi s}s}{s^2+1}
        </me>.
      </p>
      <p>
        We now use <xref ref="thm_shifting-t">Theorem</xref>
        and the facts that <m>\frac{1}{s}</m> and
        <m>\frac{s}{s^2+1}</m> are the transforms of <m>1</m> and <m>\cos t</m>,
        respectively.
        The solution <m>y(t)</m> computes as follows:
        <me>
          y(t) = \mathcal{L}^{-1}(\frac{e^{-\pi s}}{s}) - \mathcal{L}^{-1}(\frac{e^{-\pi s}s}{s^2+1}) = U_{\pi}(t) - U_{\pi}(t) \cos (t-\pi)
        </me>,
        which can be written in the more familiar form:
        <me>
          y(t) = \begin{cases} \; 0 \amp  \text{ for }   t \lt  \pi, \\ 1-\cos t \amp  \text{ for }   t>\pi. \end{cases}
        </me>
      </p>
    </solution>
  </example>
  <exercises>
    <title>Exercises for <xref ref="sec_shifting-thms">Section</xref></title>
    <exercise>
      <p>
        Find <m>\mathcal{L}(e^{t}-te^{t})</m>.
      </p>
    </exercise>
    <exercise>
      <p>
        Find <m>\mathcal{L}(e^{-4t}\sin 3t)</m>.
      </p>
    </exercise>
    <exercise>
      <p>
        Show that <m>\mathcal{L}(e^{at}\cos bt) =\frac{s-a}{(s-a)^2+b^2}</m>.
      </p>
    </exercise>
    <exercise>
      <p>
        Show that <m>\mathcal{L}(e^{at}\sin bt) =\frac{b}{( s-a)^2+b^2}</m>.
      </p>
    </exercise>
    <exercise>
      <p>
        Find <m>\mathcal{L}^{-1}(F(s))</m> for the following:
      </p>
      <ol>
        <li>
          <p>
            <m>F(s) =\frac{s+2}{s^2+4s+5}</m>.
          </p>
        </li>
        <li>
          <p>
            <m>F(s) =\frac{8}{s^2-2s+5}</m>.
          </p>
        </li>
        <li>
          <p>
            <m>F(s) =\frac{s+3}{(s+2)^2+1}</m>.
          </p>
        </li>
        <li>
          <p>
            <m>F(s) =\frac{2s+10}{s^2+6s+25}</m>.
          </p>
        </li>
      </ol>
    </exercise>
    <exercise>
      <p>
        Find <m>\mathcal{L}(\,f(t))</m> for the following:
        <ol>
          <li>
            <p>
              <m>f(t) = U_2(t)(t-2)^2</m>.
            </p>
          </li>
          <li>
            <p>
              <m>f(t) = U_1(t)e^{1-t}</m>.
            </p>
          </li>
          <li>
            <p>
              <m>f(t) = U_{3\pi}(t) \sin(t-3\pi)</m>.
            </p>
          </li>
          <li>
            <p>
              <m>f(t) = 2U_1(t) - U_2(t) - U_3(t)</m>
            </p>
          </li>
          <li>
            <p>
              Let <m>f(t)</m> be the function given in <xref ref="fig_ch-11-25">Figure</xref>.
              <figure xml:id="fig_ch-11-25">
                <caption>The graph <m>y=f(t)</m> (for Problem 6e)</caption>
                <image width="73%" source="figs/ch-11/ch-11-fig-25.pdf"/>
              </figure>
            </p>
          </li>
          <li>
            <p>
              Let <m>f(t)</m> be the function given in <xref ref="fig_ch-11-26">Figure</xref>.
              <em>Hint:</em> The function is the integral of the one in Exercise 13.
              <figure xml:id="fig_ch-11-26">
                <caption>The graph <m>y=f(t)</m> (for Problem 6f)</caption>
                <image width="73%" source="figs/ch-11/ch-11-fig-26.pdf"/>
              </figure>
            </p>
          </li>
        </ol>
      </p>
    </exercise>
    <exercise>
      <p>
        Find <m>\mathcal{L}^{-1}(\frac{e^{-s}+e^{-2s}}{s})</m>.
      </p>
    </exercise>
    <exercise>
      <p>
        Find <m>\mathcal{L}^{-1}(\frac{1-e^{-s}+e^{-2s}}{s^2})</m>.
      </p>
    </exercise>
    <exercise>
      <p>
        Solve the initial value problem for each of the following:
        <ol>
          <li>
            <p>
              <m>y^{\prime \prime}(t) + 2y\,'(t) + 2y(t) = 0</m>,
              with <m>y(0) = -1</m> and <m>y'(0) = 1</m>.
            </p>
          </li>
          <li>
            <p>
              <m>y^{\prime \prime}(t) + 4y\,'(t) + 5y(t) = 0</m>,
              with <m>y(0) = 1</m> and <m>y'(0) = -2</m>.
            </p>
          </li>
          <li>
            <p>
              <m>2y^{\prime \prime}(t) + 2y\,'(t) + y(t) = 0</m>,
              with <m>y(0) =0</m> and <m>y'(0) = 1</m>.
            </p>
          </li>
          <li>
            <p>
              <m>y^{\prime \prime}(t) - 2y\,'(t) + y(t) = 2</m>e<m>^{t}</m>,
              with <m>y(0) = 0</m> and <m>y'(0) = 0</m>.
            </p>
          </li>
          <li>
            <p>
              <m>y^{\prime \prime}(t) + 2y\,'(t) + y(t) = 6te^{-t}</m>,
              with <m>y(0) = 0</m> and <m>y'(0) = 0</m>.
            </p>
          </li>
          <li>
            <p>
              <m>y^{\prime \prime}(t) + 2y\,'(t) + y(t) = 2U_1(t)e^{1-t}</m>,
              with <m>y(0) =0</m> and <m>y'(0) = 0</m>.
            </p>
          </li>
          <li>
            <p>
              <m>y^{\prime \prime}(t) + y(t) = U_{\pi /2}(t)</m>,
              with <m>y(0) = 0</m> and <m>y'(0) = 1</m>.
            </p>
          </li>
        </ol>
      </p>
    </exercise>
  </exercises>
</section>